more proof

Weidenbach_Book/Watched_Literals/Watched_Literals_Algorithm_Restart.thy
@@ -1,5 +1,6 @@
 theory Watched_Literals_Algorithm_Restart
-  imports Watched_Literals_Algorithm Watched_Literals_Transition_System_Restart
+imports Watched_Literals_Algorithm Watched_Literals_Transition_System_Restart
+  "../../lib/Explorer"
 begin
 
 context twl_restart_ops
@@ -14,7 +15,7 @@ definition (in -) restart_prog_pre :: \<open>'v twl_st \<Rightarrow> bool \<Righ
     (\<not>brk \<longrightarrow> get_conflict S = None)\<close>
 
 definition restart_prog
-  :: "'v twl_st \<Rightarrow> nat \<Rightarrow> nat \<Rightarrow> bool \<Rightarrow> ('v twl_st \<times> nat \<times> nat) nres"
+  :: \<open>'v twl_st \<Rightarrow> nat \<Rightarrow> nat \<Rightarrow> bool \<Rightarrow> ('v twl_st \<times> nat \<times> nat) nres\<close>
 where
   \<open>restart_prog S m n brk = do {
      ASSERT(restart_prog_pre S brk);
@@ -35,33 +36,228 @@ where
        RETURN (S, m, n)
    }\<close>
 
-definition cdcl_twl_stgy_restart_prog_inv where
-  \<open>cdcl_twl_stgy_restart_prog_inv S\<^sub>0 brk T m n \<longleftrightarrow> twl_struct_invs T \<and> twl_stgy_invs T \<and>
+fun cdcl_twl_stgy_restart_prog_inv where
+  \<open>cdcl_twl_stgy_restart_prog_inv S\<^sub>0 (brk, S, T, m, n) \<longleftrightarrow>
+    twl_struct_invs S\<^sub>0 \<and>
+    twl_struct_invs T \<and> twl_stgy_invs T \<and>
     (brk \<longrightarrow> final_twl_state T) \<and>
-    cdcl_twl_stgy_restart_with_leftovers (S\<^sub>0, 0, True) m (T, n, True) \<and>
+    cdcl_twl_stgy_restart_with_leftovers (S\<^sub>0, 0, True) m S (T, n, True) \<and>
     clauses_to_update T = {#} \<and> (\<not>brk \<longrightarrow> get_conflict T = None)\<close>
 
-lemma
-  \<open>wf {((brk, T, m, n), (brk', S\<^sub>0, m', n')).
-       twl_struct_invs T \<and> twl_stgy_invs T \<and>
-    cdcl_twl_stgy_restart_with_leftovers (S\<^sub>0, 0, True) m (T, n, True)}\<close>
-  oops
+lemmas cdcl_twl_stgy_restart_prog_inv_def[simp del] =
+  cdcl_twl_stgy_restart_prog_inv.simps
 
 definition cdcl_twl_stgy_restart_prog :: "'v twl_st \<Rightarrow> 'v twl_st nres" where
   \<open>cdcl_twl_stgy_restart_prog S\<^sub>0 =
   do {
-    (brk, T, _, _) \<leftarrow> WHILE\<^sub>T\<^bsup>\<lambda>(brk, T, m, n). cdcl_twl_stgy_restart_prog_inv S\<^sub>0 brk T m n\<^esup>
+    (brk, T, _, _, _) \<leftarrow> WHILE\<^sub>T\<^bsup>cdcl_twl_stgy_restart_prog_inv S\<^sub>0\<^esup>
       (\<lambda>(brk, _). \<not>brk)
-      (\<lambda>(brk, S, m, n).
+      (\<lambda>(brk, S, S', m, n).
       do {
         T \<leftarrow> unit_propagation_outer_loop S;
         (brk, T) \<leftarrow> cdcl_twl_o_prog T;
-        (T, m, n) \<leftarrow> restart_prog T m n brk;
-        RETURN (brk, T, m, n)
+        (T, m', n') \<leftarrow> restart_prog T m n brk;
+        RETURN (brk, T, T, m', n')
       })
-      (False, S\<^sub>0, size (get_all_learned_clss S\<^sub>0), 0);
+      (False, S\<^sub>0, S\<^sub>0, size (get_all_learned_clss S\<^sub>0), 0);
     RETURN T
   }\<close>
+end
+
+context twl_restart
+begin
+
+
+lemma restart_prog_spec:
+  assumes
+    inv: \<open>cdcl_twl_stgy_restart_prog_inv S (brkU, U, T, m, n)\<close> and
+    cond: \<open>case (brkU, U, T, m, n) of (brk, uu_) \<Rightarrow> \<not> brk\<close> and
+    other_inv: \<open>cdcl_twl_o_prog_spec V (brkT, W)\<close> and
+    struct_invs_V: \<open>twl_struct_invs V\<close> and
+    cp: \<open>cdcl_twl_cp\<^sup>*\<^sup>* U V\<close> and
+    lits_to_update: \<open>literals_to_update V = {#}\<close> and
+    \<open>\<forall>S'. \<not> cdcl_twl_cp V S'\<close> and
+    \<open>twl_stgy_invs V\<close>
+  shows \<open>restart_prog W m n brkT
+         \<le> SPEC
+            (\<lambda>x. (case x of
+                  (Ta, m', n') \<Rightarrow>
+                    RETURN (brkT, Ta, Ta, m', n'))
+                 \<le> SPEC
+                    (\<lambda>s'. cdcl_twl_stgy_restart_prog_inv S s' \<and>
+                          (s', brkU, U, T, m, n)
+                          \<in> {((brkT, T, T', n, n'), brkS, S, S', m, m').
+                             twl_struct_invs S \<and>
+                             \<not> brkS \<and>
+                             cdcl_twl_stgy_restart_with_leftovers1
+                              (S, m', \<not>brkS) (T, n', \<not>brkT)} \<union>
+                            {((brkT, T), brkS, S). S = T \<and> brkT \<and> \<not> brkS}))\<close>
+proof -
+  have [simp]: \<open>\<not>brkU\<close>
+    using cond by auto
+  have struct_invs': \<open>cdcl_twl_restart W T' \<Longrightarrow> cdcl_twl_stgy\<^sup>*\<^sup>* T' V' \<Longrightarrow> twl_struct_invs V'\<close> for T' V'
+    using assms(3) cdcl_twl_restart_twl_struct_invs
+    by (metis (no_types, lifting) case_prodD rtranclp_cdcl_twl_stgy_twl_struct_invs)
+  have stgy_invs: \<open>cdcl_twl_restart W V' \<Longrightarrow> cdcl_twl_stgy\<^sup>*\<^sup>* V' W' \<Longrightarrow> twl_stgy_invs W'\<close> for V' W'
+    using assms(3) cdcl_twl_restart_twl_stgy_invs
+    by (metis (no_types, lifting) case_prodD cdcl_twl_restart_twl_struct_invs
+      rtranclp_cdcl_twl_stgy_twl_stgy_invs)
+  have res_no_clss_to_upd: \<open>cdcl_twl_restart U V \<Longrightarrow> clauses_to_update V = {#}\<close> for V
+    by (auto simp: cdcl_twl_restart.simps)
+  have res_no_confl: \<open>cdcl_twl_restart U V \<Longrightarrow> get_conflict V = None\<close> for V
+    by (auto simp: cdcl_twl_restart.simps)
+
+  have
+    struct_invs_S: \<open>twl_struct_invs S\<close> and
+    struct_invs_T: \<open>twl_struct_invs T\<close> and
+    twl_stgy_invs_T: \<open>twl_stgy_invs T\<close> and
+    \<open>brkU \<longrightarrow> final_twl_state T\<close> and
+    twl_res: \<open>cdcl_twl_stgy_restart_with_leftovers (S, 0, True) m U (T, n, True)\<close> and
+    clss_T: \<open>clauses_to_update T = {#}\<close> and
+    confl: \<open>\<not> brkU \<longrightarrow> get_conflict T = None\<close>
+    using inv unfolding cdcl_twl_stgy_restart_prog_inv_def prod.case by fast+
+  have
+    cdcl_o: \<open>cdcl_twl_o\<^sup>*\<^sup>* V W\<close> and
+    conflict_W: \<open>get_conflict W \<noteq> None \<Longrightarrow> count_decided (get_trail W) = 0\<close> and
+    brk'_no_step: \<open>brkT \<Longrightarrow> final_twl_state W\<close> and
+    struct_invs_W: \<open>twl_struct_invs W\<close> and
+    stgy_invs_W: \<open>twl_stgy_invs W\<close> and
+    clss_to_upd_W: \<open>clauses_to_update W = {#}\<close> and
+    lits_to_upd_W: \<open>\<not> brkT \<longrightarrow> literals_to_update W \<noteq> {#}\<close> and
+    confl_W: \<open>\<not> brkT \<longrightarrow> get_conflict W = None\<close>
+    using other_inv unfolding final_twl_state_def by fast+
+
+  have \<open>cdcl_twl_stgy\<^sup>*\<^sup>* V W\<close>
+    by (meson cdcl_o assms(5) rtranclp_cdcl_twl_cp_stgyD rtranclp_cdcl_twl_o_stgyD
+        rtranclp_trans)
+  from twl_res have
+    STa: \<open>cdcl_twl_stgy_restart\<^sup>*\<^sup>* (S, 0, True) (U, n, True)\<close> and
+    TaT: \<open>cdcl_twl_stgy\<^sup>*\<^sup>* U T\<close> and
+    m: \<open>m = size (get_all_learned_clss U)\<close>
+    unfolding cdcl_twl_stgy_restart_with_leftovers_def prod.case snd_conv fst_conv
+    by blast+
+
+  have restart_prog_pre_W: \<open>restart_prog_pre W brkT\<close>
+    using confl_W stgy_invs_W struct_invs_W
+    unfolding restart_prog_pre_def
+    by fast
+  have struct_invs_U: \<open>twl_struct_invs U\<close>
+    using rtranclp_cdcl_twl_stgy_restart_twl_struct_invs[OF STa] struct_invs_S
+    by simp
+
+  have UW: \<open>cdcl_twl_stgy\<^sup>*\<^sup>* U W\<close>
+    by (meson \<open>cdcl_twl_stgy\<^sup>*\<^sup>* V W\<close> local.cp rtranclp_cdcl_twl_cp_stgyD rtranclp_trans)
+  have only_restart: \<open>cdcl_twl_stgy_restart_prog_inv S
+       (False, Y, Y, size (get_all_learned_clss Y), n)\<close> (is ?A) and
+     only_restart_term: \<open>((False, Y, Y, size (get_all_learned_clss Y), n),
+        brkU, U, T, m, n)
+        \<in> {((brkT, T, T', n, n'), brkS, S, S', m, m').
+        twl_struct_invs S \<and>
+        \<not> brkS \<and>
+        cdcl_twl_stgy_restart_with_leftovers1 (S, m', \<not>brkS) (T, n', \<not>brkT)} \<union>
+        {((brkT, T), brkS, S). S = T \<and> brkT \<and> \<not> brkS}\<close> (is ?B)
+    if
+      \<open>True \<longrightarrow> f n < size (get_all_learned_clss W) - m\<close> and
+      m_size_W: \<open>True \<longrightarrow> m < size (get_all_learned_clss W)\<close> and
+      WY: \<open>cdcl_twl_restart_only W Y\<close> and
+      brkX and
+      X and
+      \<open>\<not> brkT\<close>
+    for X brkX Y
+  proof -
+    have \<open>twl_struct_invs Y\<close>
+      using WY cdcl_twl_restart_only_twl_struct_invs struct_invs_W by blast
+    moreover have \<open>twl_stgy_invs Y\<close>
+      using WY cdcl_twl_stgy_restart_only_twl_stgy_invs stgy_invs_W by blast
+    moreover have \<open>clauses_to_update Y = {#}\<close> \<open>get_conflict Y = None\<close>
+      using WY by (auto simp: cdcl_twl_restart_only.simps)
+    moreover {
+      have \<open>cdcl_twl_stgy_restart (U, n, True) (Y, n, True)\<close>
+        apply (rule restart_noGC[OF _ _ WY])
+        unfolding m[symmetric]
+        defer
+        apply (auto simp: m_size_W UW)[]
+        by (metis (mono_tags, hide_lams) Nitpick.rtranclp_unfold \<open>cdcl_twl_stgy\<^sup>*\<^sup>* V W\<close> UW lits_to_upd_W
+          lits_to_update local.cp that(6) tranclp_cdcl_twl_cp_stgyD tranclp_rtranclp_tranclp)
+      then have \<open>cdcl_twl_stgy_restart_with_leftovers (S, 0, True)
+        (size (get_all_learned_clss Y)) Y (Y, n, True)\<close>
+        using STa
+        unfolding cdcl_twl_stgy_restart_with_leftovers_def
+        by auto
+    }
+    ultimately show ?A
+      using struct_invs_S
+      unfolding cdcl_twl_stgy_restart_prog_inv_def
+      by auto
+    have \<open>cdcl_twl_stgy_restart_with_leftovers1 (U, n, True) (Y, n, True)\<close>
+      using m_size_W
+      unfolding cdcl_twl_stgy_restart_with_leftovers1_def m
+      apply (auto intro!: cdcl_twl_stgy_restart.intros(2)[of _ W] simp: WY)[]
+      by (metis Nitpick.rtranclp_unfold UW nat_neq_iff)
+    then show ?B by (auto simp: struct_invs_U m)
+  qed
+  have full_restart: \<open>cdcl_twl_stgy_restart_prog_inv S (False, Z, Z, size (get_all_learned_clss Z), n + 1)\<close> (is ?A)and
+    full_restart_term:
+      \<open>((False, Z, Z, size (get_all_learned_clss Z), n + 1), brkU, U, T, m, n)
+    \<in> {((brkT, T, T', n, n'), brkS, S, S', m, m').
+       twl_struct_invs S \<and>
+       \<not> brkS \<and>
+       cdcl_twl_stgy_restart_with_leftovers1 (S, m', \<not> brkS)
+        (T, n', \<not> brkT)} \<union>
+      {((brkT, T), brkS, S). S = T \<and> brkT \<and> \<not> brkS}\<close> (is ?B)
+    if
+      \<open>restart_prog_pre W False\<close> and
+      m_size: \<open>True \<longrightarrow> f n < size (get_all_learned_clss W) - m\<close> and
+      \<open>True \<longrightarrow> m < size (get_all_learned_clss W)\<close> and
+      \<open>\<not> (brkX \<and> True \<and> \<not> False)\<close> and
+      WY: \<open>cdcl_twl_restart W Y\<close> and
+      X and
+      \<open>\<not> brkT\<close> and
+      YZ: \<open>cdcl_twl_stgy\<^sup>*\<^sup>* Y Z\<close> and
+      clss_Z: \<open>clauses_to_update Z = {#}\<close> and
+      confl_Z: \<open>get_conflict Z = None\<close>
+    for X brkX Y Z
+  proof -
+    have UW: \<open>cdcl_twl_stgy\<^sup>+\<^sup>+ U W\<close>
+      by (metis (mono_tags) Nitpick.rtranclp_unfold \<open>cdcl_twl_stgy\<^sup>*\<^sup>* V W\<close> lits_to_upd_W
+        lits_to_update local.cp that(7) tranclp_cdcl_twl_cp_stgyD tranclp_rtranclp_tranclp)
+    have UZ: \<open>cdcl_twl_stgy_restart (U, n, True) (Z, Suc n, True)\<close>
+      apply (rule restart_step[OF UW _ WY YZ])
+      using m_size
+      unfolding m[symmetric]
+      by (auto simp: m UW clss_Z confl_Z)
+    have \<open>twl_struct_invs Z\<close>
+      using struct_invs' WY YZ by blast
+    moreover have \<open>twl_stgy_invs Z\<close>
+      using WY YZ stgy_invs by blast
+    moreover have \<open>cdcl_twl_stgy_restart_with_leftovers (S, 0, True)
+        (size (get_all_learned_clss Z)) Z (Z, Suc n, True)\<close>
+        using STa UZ
+        by (auto simp: cdcl_twl_stgy_restart_with_leftovers_def)
+    ultimately show ?A
+      using struct_invs_S YZ WY clss_Z confl_Z
+      unfolding cdcl_twl_stgy_restart_prog_inv_def
+      by auto
+    have \<open>cdcl_twl_stgy_restart_with_leftovers1 (U, n, True) (Z, Suc n, True)\<close>
+      using UZ by (auto simp: cdcl_twl_stgy_restart_with_leftovers1_def)
+    then show ?B
+      by (auto simp: struct_invs_U)
+  qed
+  show ?thesis
+    unfolding restart_prog_def restart_required_def
+    apply (refine_vcg; remove_dummy_vars)
+    subgoal by (rule restart_prog_pre_W)
+    subgoal for X brkX Y
+      by (rule only_restart)
+    subgoal for X brkX Y
+      by (rule only_restart_term)
+    subgoal for X brkX Y Z
+      by (rule full_restart)
+    subgoal for X brkX Y Z
+      by (rule full_restart_term)
+    subgoal for X brkX
+        
+qed
 
 lemma (in twl_restart)
   assumes
@@ -85,7 +281,7 @@ lemma (in twl_restart)
     twl_struct_invs T \<and>
     twl_stgy_invs T \<and>
     (brk \<longrightarrow> final_twl_state T) \<and>
-    cdcl_twl_stgy_restart_with_leftovers (S, 0, \<not>brk) m (T, n'', \<not>brk) \<and>
+    cdcl_twl_stgy_restart_with_leftovers (S, 0, \<not>brk) m S (T, n'', \<not>brk) \<and>
     clauses_to_update T = {#} \<and>
     (\<not> brk \<longrightarrow> get_conflict T = None)) \<and>
  (s', brk, T, n)
@@ -202,7 +398,7 @@ proof -
     cdcl_twl_stgy_restart_with_leftovers_after_restart_T_V:
       \<open>cdcl_twl_stgy_restart_with_leftovers (Ta, n, \<not>False) (?m V) (V, n, \<not>False)\<close> and
     cdcl_twl_stgy_restart_with_leftovers1_after_restart_only:
-      \<open>cdcl_twl_stgy_restart_with_leftovers1 (Ta, n, \<not>False) (V, n, \<not>False)\<close>
+    \<open>cdcl_twl_stgy_restart_with_leftovers1 (Ta, n, \<not>False) (V, n, \<not>False)\<close>
     if
       f: \<open>True \<longrightarrow> m < size (get_all_learned_clss U)\<close> and
       res: \<open>cdcl_twl_restart_only U V\<close> and
@@ -321,6 +517,403 @@ proof -
     subgoal by (auto simp add: cdcl_twl_restart_only.simps)
     subgoal apply (auto intro!: struct_invs_S struct_invs_T
       cdcl_twl_stgy_restart_with_leftovers1_after_restart_only[unfolded not_False_eq_True])
+thm 
+  cdcl_twl_stgy_restart_with_leftovers1_after_restart_only[unfolded not_False_eq_True]
+
+      apply (rule 
+        cdcl_twl_stgy_restart_with_leftovers1_after_restart_only[unfolded not_False_eq_True])
+      sorry
+    subgoal by (rule struct_invs')
+    subgoal by (rule stgy_invs)
+    subgoal by simp
+    subgoal
+      by (rule cdcl_twl_stgy_restart_with_leftovers_after_restart, simp)
+    subgoal
+      using rtranclp_twl_restart_after_restart_T_U
+      by (auto intro!: struct_invs_S struct_invs_T
+        cdcl_twl_stgy_restart_with_leftovers1_after_restart[unfolded not_False_eq_True])
+    subgoal by (rule struct_invs_U)
+    subgoal by (rule stgy_invs_U)
+    subgoal by (rule brk'_no_step) simp
+    subgoal
+      by (auto intro: rtranclp_twl_restart_after_restart_brk
+        rtranclp_twl_restart_after_restart_S_U)
+    subgoal by (rule clss_to_upd_U)
+    subgoal using struct_invs_U conflict_U lits_to_upd_U
+      by (cases \<open>get_conflict U\<close>)(auto simp: twl_struct_invs_def)
+    subgoal
+      using cdcl_twl_stgy_restart_with_leftovers1_T_U brk'_eq
+      by (auto simp: twl_restart_after_restart struct_invs_S struct_invs_T
+        cdcl_twl_stgy_restart_with_leftovers_after_restart_T_V struct_invs_U
+        rtranclp_twl_restart_after_restart_brk rtranclp_twl_restart_after_restart_T_U
+        cdcl_twl_stgy_restart_with_leftovers1_after_restart)
+    done
+qed
+
+lemma (in twl_restart) cdcl_twl_stgy_restart_prog_spec:
+  fixes S :: \<open>'v twl_st\<close>
+  assumes \<open>twl_struct_invs S\<close> and \<open>twl_stgy_invs S\<close> and \<open>clauses_to_update S = {#}\<close> and
+    \<open>get_conflict S = None\<close>
+  shows
+    \<open>cdcl_twl_stgy_restart_prog S \<le> SPEC(\<lambda>T.
+       \<exists>S' m n. cdcl_twl_stgy_restart_with_leftovers (S, 0, True) m S' (T, n, True) \<and>
+        final_twl_state T)\<close>
+    (is \<open>_ \<le> SPEC(\<lambda>T. ?P T)\<close>)
+proof -
+  
+  (* have final_prop: \<open>?P T\<close>
+   *   if
+   *    inv: \<open>case (brk, T, n) of  (brk, T, m, n) \<Rightarrow> cdcl_twl_stgy_restart_prog_inv S brk T m n\<close> and
+   *     \<open>\<not> (case (brk, T, n) of (brk, uu_) \<Rightarrow> \<not> brk)\<close>
+   *   for brk T n
+   * proof -
+   *   have
+   *     \<open>brk\<close> and
+   *     \<open>twl_struct_invs T\<close> and
+   *     \<open>twl_stgy_invs T\<close> and
+   *     ns: \<open>final_twl_state T\<close> and
+   *     twl_left_overs: \<open>cdcl_twl_stgy_restart_with_leftovers (S, 0) (T, n)\<close> and
+   *     \<open>clauses_to_update T = {#}\<close>
+   *     using that unfolding cdcl_twl_stgy_restart_prog_inv_def by auto
+   *   obtain S' where
+   *      st: \<open>cdcl_twl_stgy_restart\<^sup>*\<^sup>* (S, 0) (S', n)\<close> and
+   *      S'_T: \<open>cdcl_twl_stgy\<^sup>*\<^sup>* S' T\<close>
+   *     using twl_left_overs unfolding cdcl_twl_stgy_restart_with_leftovers_def by auto
+   *   then show ?thesis
+   *     using ns unfolding cdcl_twl_stgy_restart_with_leftovers_def apply -
+   *     apply (rule_tac x=n in exI)
+   *     apply (rule conjI)
+   *     subgoal by (rule_tac x=S' in exI) auto
+   *     subgoal by auto
+   *     done
+  * qed *)
+  let ?R = \<open>{((brkT :: bool, T :: 'v twl_st, T' :: 'v twl_st, n :: nat, n' :: nat),
+      brkS, S, S' :: 'v twl_st, m :: nat, m' :: nat).
+    twl_struct_invs S \<and> \<not> brkS \<and>
+    cdcl_twl_stgy_restart_with_leftovers1 (S, m, brkS) (T, n, brkT)} \<union>
+    {((brkT, T), brkS, S). S = T \<and> brkT \<and> \<not> brkS}\<close>
+
+  have wf: \<open>wf ?R\<close>
+    apply (rule wf_union_compatible)
+    subgoal
+      by (rule wf_if_measure_in_wf[OF wf_cdcl_twl_stgy_restart_with_leftovers1,
+          of _  \<open>\<lambda>(brkT, T, T', n, n'). (T, n, brkT)\<close>])
+        auto
+    subgoal
+      by (rule wf_no_loop) auto
+    subgoal
+      by auto
+    done
+   term cdcl_twl_stgy_restart
+
+  show ?thesis
+    supply RETURN_as_SPEC_refine[refine2 del]
+    unfolding cdcl_twl_stgy_restart_prog_def full_def
+    apply (refine_vcg WHILEIT_rule[where R = \<open>?R\<close>];
+      remove_dummy_vars)
+    subgoal by (rule wf)
+    subgoal using assms unfolding cdcl_twl_stgy_restart_prog_inv_def cdcl_twl_stgy_restart_with_leftovers_def
+      by auto
+    subgoal using assms unfolding cdcl_twl_stgy_restart_prog_inv_def cdcl_twl_stgy_restart_with_leftovers_def
+      by (auto dest: rtranclp_cdcl_twl_stgy_restart_twl_struct_invs)
+    subgoal using assms
+      by (auto simp: cdcl_twl_stgy_restart_prog_inv_def cdcl_twl_stgy_restart_with_leftovers_def
+        dest!: rtranclp_cdcl_twl_stgy_restart_clauses_to_update)
+    subgoal using assms
+      by (auto simp: cdcl_twl_stgy_restart_prog_inv_def cdcl_twl_stgy_restart_with_leftovers_def
+        dest!: rtranclp_cdcl_twl_stgy_restart_get_conflict)
+    subgoal
+      using assms
+      by (auto simp: cdcl_twl_stgy_restart_prog_inv_def cdcl_twl_stgy_restart_with_leftovers_def
+        dest: rtranclp_cdcl_twl_stgy_restart_twl_stgy_invs)
+    subgoal
+      using assms
+      by (auto simp: cdcl_twl_stgy_restart_prog_inv_def cdcl_twl_stgy_restart_with_leftovers_def
+        no_step_cdcl_twl_cp_no_step_cdcl\<^sub>W_cp)
+    subgoal by fast
+    subgoal for brkU U T m n V brkT W
+      explore_lemma
+      sorry
+
+    subgoal by (rule wf_cdcl_twl_stgy_restart_measure)
+    subgoal using assms by fast
+    subgoal using assms by fast
+    subgoal using assms by fast
+    subgoal by (rule cdcl_twl_stgy_restart_with_leftovers_refl)
+    subgoal using assms by fast
+    subgoal using assms by fast
+    subgoal by fast
+    subgoal by fast
+    subgoal by fast
+    subgoal by fast
+    subgoal by (simp add: no_step_cdcl_twl_cp_no_step_cdcl\<^sub>W_cp)
+    subgoal by fast
+    subgoal by (rule final_prop[unfolded cdcl_twl_stgy_restart_prog_inv_def])
+    done
+qed
+lemma (in twl_restart)
+  assumes
+    inv: \<open>case (brk, T, m, n) of  (brk, T, m, n) \<Rightarrow> cdcl_twl_stgy_restart_prog_inv S brk T m n\<close> and
+    cond: \<open>case (brk, T, m, n) of (brk, uu_) \<Rightarrow> \<not> brk\<close> and
+    other_inv: \<open>cdcl_twl_o_prog_spec S' (brk', U)\<close> and
+    struct_invs_S: \<open>twl_struct_invs S'\<close> and
+    cp: \<open>cdcl_twl_cp\<^sup>*\<^sup>* T S'\<close> and
+    lits_to_update: \<open>literals_to_update S' = {#}\<close> and
+    \<open>\<forall>S'a. \<not> cdcl_twl_cp S' S'a\<close> and
+    \<open>twl_stgy_invs S'\<close> and
+    brk: \<open>(brk', brk) \<in> bool_rel\<close>
+  shows restart_prog_spec:
+    \<open>restart_prog U m n brk'
+         \<le> SPEC
+             (\<lambda>x. (case x of
+                   (T, m, na) \<Rightarrow> RETURN (brk', T, m, na))
+                  \<le> SPEC
+                      (\<lambda>s'. (case s' of
+  (brk, T, m, n'') \<Rightarrow>
+    twl_struct_invs T \<and>
+    twl_stgy_invs T \<and>
+    (brk \<longrightarrow> final_twl_state T) \<and>
+    cdcl_twl_stgy_restart_with_leftovers (S, 0, \<not>brk) m S (T, n'', \<not>brk) \<and>
+    clauses_to_update T = {#} \<and>
+    (\<not> brk \<longrightarrow> get_conflict T = None)) \<and>
+ (s', brk, T, n)
+ \<in> {((brkT, T, m, n'), brkS, S, _).
+     twl_struct_invs S \<and>
+     cdcl_twl_stgy_restart_with_leftovers1 (S, n, \<not>brkS) (T, n', \<not>brkS)} \<union>
+    {((brkT, T, _, _), brkS, S, _). S = T \<and> brkT \<and> \<not> brkS}))\<close> (is ?A)
+proof -
+  have brk[simp]: \<open>brk' = brk\<close>
+    using brk by auto
+  have struct_invs': \<open>cdcl_twl_restart U T \<Longrightarrow> cdcl_twl_stgy\<^sup>*\<^sup>* T V \<Longrightarrow> twl_struct_invs V\<close> for T V
+    using assms(3) cdcl_twl_restart_twl_struct_invs
+    by (metis (no_types, lifting) case_prodD rtranclp_cdcl_twl_stgy_twl_struct_invs)
+  have stgy_invs: \<open>cdcl_twl_restart U V \<Longrightarrow> cdcl_twl_stgy\<^sup>*\<^sup>* V W \<Longrightarrow> twl_stgy_invs W\<close> for V W
+    using assms(3) cdcl_twl_restart_twl_stgy_invs
+    by (metis (no_types, lifting) case_prodD cdcl_twl_restart_twl_struct_invs
+      rtranclp_cdcl_twl_stgy_twl_stgy_invs)
+  have res_no_clss_to_upd: \<open>cdcl_twl_restart U V \<Longrightarrow> clauses_to_update V = {#}\<close> for V
+    by (auto simp: cdcl_twl_restart.simps)
+  have res_no_confl: \<open>cdcl_twl_restart U V \<Longrightarrow> get_conflict V = None\<close> for V
+    by (auto simp: cdcl_twl_restart.simps)
+
+  have
+    struct_invs_T: \<open>twl_struct_invs T\<close> and
+    \<open>twl_stgy_invs T\<close> and
+    \<open>brk \<longrightarrow> final_twl_state T\<close> and
+    twl_res: \<open>cdcl_twl_stgy_restart_with_leftovers (S, 0, True) m (T, n, True)\<close> and
+    \<open>clauses_to_update T = {#}\<close> and
+    confl: \<open>\<not> brk \<longrightarrow> get_conflict T = None\<close>
+    using inv unfolding cdcl_twl_stgy_restart_prog_inv_def prod.case by fast+
+  have
+    cdcl_o: \<open>cdcl_twl_o\<^sup>*\<^sup>* S' U\<close> and
+    conflict_U: \<open>get_conflict U \<noteq> None \<Longrightarrow> count_decided (get_trail U) = 0\<close> and
+    brk'_no_step: \<open>brk' \<Longrightarrow> final_twl_state U\<close> and
+    struct_invs_U: \<open>twl_struct_invs U\<close> and
+    stgy_invs_U: \<open>twl_stgy_invs U\<close> and
+    clss_to_upd_U: \<open>clauses_to_update U = {#}\<close> and
+    lits_to_upd_U: \<open>\<not> brk' \<longrightarrow> literals_to_update U \<noteq> {#}\<close> and
+    confl_U: \<open>\<not> brk' \<longrightarrow> get_conflict U = None\<close>
+    using other_inv unfolding final_twl_state_def by fast+
+
+  have \<open>cdcl_twl_stgy\<^sup>*\<^sup>* T U\<close>
+    by (meson \<open>cdcl_twl_o\<^sup>*\<^sup>* S' U\<close> assms(5) rtranclp_cdcl_twl_cp_stgyD rtranclp_cdcl_twl_o_stgyD
+        rtranclp_trans)
+  from twl_res obtain Ta where
+    STa: \<open>cdcl_twl_stgy_restart\<^sup>*\<^sup>* (S, 0, True) (Ta, n, True)\<close> and
+    TaT: \<open>cdcl_twl_stgy\<^sup>*\<^sup>* Ta T\<close> and
+    m: \<open>m = size (get_all_learned_clss Ta)\<close>
+    unfolding cdcl_twl_stgy_restart_with_leftovers_def prod.case snd_conv fst_conv
+    by blast
+  have
+    twl_restart_after_restart:
+      \<open>cdcl_twl_stgy_restart (Ta, n, \<not>False) (W, Suc n, \<not>False)\<close> and
+    rtranclp_twl_restart_after_restart:
+      \<open>cdcl_twl_stgy_restart\<^sup>*\<^sup>* (S, 0, \<not>False) (W, n + 1, \<not>False)\<close> and
+    cdcl_twl_stgy_restart_with_leftovers_after_restart:
+      \<open>cdcl_twl_stgy_restart_with_leftovers (S, 0, \<not>False) (size (get_all_learned_clss W))
+        (W, n + 1, \<not>False)\<close> and
+    cdcl_twl_stgy_restart_with_leftovers_after_restart_T_V:
+    \<open>cdcl_twl_stgy_restart_with_leftovers (Ta, n, \<not>False) (size (get_all_learned_clss W))
+         (W, Suc n, \<not>False)\<close> and
+    cdcl_twl_stgy_restart_with_leftovers1_after_restart:
+      \<open>cdcl_twl_stgy_restart_with_leftovers1 (Ta, n, \<not>False) (W, Suc n, \<not>False)\<close>
+    if
+      f: \<open>True \<longrightarrow> f (snd (U, n)) < size (get_all_learned_clss (fst (U, n))) - m\<close> and
+      res: \<open>cdcl_twl_restart U V\<close> and
+      pre: \<open>cdcl_twl_stgy\<^sup>*\<^sup>* V W\<close> and
+      [unfolded brk, simp]: \<open>brk' = False\<close>
+    for V W
+  proof -
+    have \<open>S' \<noteq> U\<close>
+      using lits_to_update lits_to_upd_U by auto
+    then have \<open>cdcl_twl_o\<^sup>+\<^sup>+ S' U\<close>
+      using \<open>cdcl_twl_o\<^sup>*\<^sup>* S' U\<close> unfolding rtranclp_unfold by auto
+    then have st: \<open>cdcl_twl_stgy\<^sup>+\<^sup>+ Ta U\<close>
+      using TaT
+      by (meson local.cp rtranclp_cdcl_twl_cp_stgyD rtranclp_tranclp_tranclp
+          tranclp_cdcl_twl_o_stgyD)
+
+    show twl_res_T_V[unfolded not_False_eq_True]:
+      \<open>cdcl_twl_stgy_restart (Ta, n, \<not>False) (W, Suc n, \<not>False)\<close>
+      unfolding not_False_eq_True
+      apply (rule cdcl_twl_stgy_restart.restart_step[of _ U _ V])
+      subgoal by (rule st)
+      subgoal using f unfolding m by simp
+      subgoal by (rule res)
+      subgoal using pre by simp
+      done
+    show \<open>cdcl_twl_stgy_restart_with_leftovers (Ta, n, \<not>False)
+        (size (get_all_learned_clss W)) (W, Suc n, \<not>False)\<close>
+      unfolding not_False_eq_True cdcl_twl_stgy_restart_with_leftovers_def
+      by (rule exI[of _ \<open>W\<close>])(auto simp: twl_res_T_V)
+    show \<open>cdcl_twl_stgy_restart\<^sup>*\<^sup>* (S, 0, \<not>False) (W, n + 1, \<not>False)\<close>
+      using twl_res twl_res_T_V STa
+      unfolding cdcl_twl_stgy_restart_with_leftovers_def apply -
+      by (auto dest: cdcl_twl_stgy_restart_cdcl_twl_stgy_cdcl_twl_stgy_restart)
+    then show  \<open>cdcl_twl_stgy_restart_with_leftovers (S, 0, \<not>False) (size (get_all_learned_clss W))
+        (W, n + 1, \<not>False)\<close>
+      unfolding cdcl_twl_stgy_restart_with_leftovers_def apply -
+      by (rule exI[of _ W]) auto
+    show \<open>cdcl_twl_stgy_restart_with_leftovers1 (Ta, n, \<not>False) (W, Suc n, \<not>False)\<close>
+      using twl_res_T_V
+      unfolding cdcl_twl_stgy_restart_with_leftovers1_def not_False_eq_True
+      by fast
+  qed
+  let ?m = \<open>\<lambda>W. (size (get_all_learned_clss W))\<close>
+  have
+    twl_restart_after_restart_only:
+      \<open>cdcl_twl_stgy_restart (Ta, n, \<not>False) (V, n, \<not>False)\<close> and
+    rtranclp_twl_restart_after_restart_only:
+      \<open>cdcl_twl_stgy_restart\<^sup>*\<^sup>* (S, 0, \<not>False) (V, n, \<not>False)\<close> and
+    cdcl_twl_stgy_restart_with_leftovers_after_restart_only:
+      \<open>cdcl_twl_stgy_restart_with_leftovers (S, 0, \<not>False) (?m V) (V, n, \<not>False)\<close> and
+    cdcl_twl_stgy_restart_with_leftovers_after_restart_T_V:
+      \<open>cdcl_twl_stgy_restart_with_leftovers (Ta, n, \<not>False) (?m V) (V, n, \<not>False)\<close> and
+    cdcl_twl_stgy_restart_with_leftovers1_after_restart_only:
+    \<open>cdcl_twl_stgy_restart_with_leftovers1 (Ta, n, \<not>False) (V, n, \<not>False)\<close>
+    if
+      f: \<open>True \<longrightarrow> m < size (get_all_learned_clss U)\<close> and
+      res: \<open>cdcl_twl_restart_only U V\<close> and
+      [unfolded brk, simp]: \<open>brk' = False\<close>
+    for V
+  proof -
+    have \<open>S' \<noteq> U\<close>
+      using lits_to_update lits_to_upd_U by auto
+    then have \<open>cdcl_twl_o\<^sup>+\<^sup>+ S' U\<close>
+      using \<open>cdcl_twl_o\<^sup>*\<^sup>* S' U\<close> unfolding rtranclp_unfold by auto
+    then have st: \<open>cdcl_twl_stgy\<^sup>+\<^sup>+ Ta U\<close> and st2: \<open>cdcl_twl_stgy\<^sup>+\<^sup>+ T U\<close>
+      using TaT
+      by (meson local.cp rtranclp_cdcl_twl_cp_stgyD rtranclp_tranclp_tranclp
+          tranclp_cdcl_twl_o_stgyD)+
+
+    show twl_res_T_V[unfolded not_False_eq_True]:
+      \<open>cdcl_twl_stgy_restart (Ta, n, \<not>False) (V, n, \<not>False)\<close>
+      unfolding not_False_eq_True
+      apply (rule cdcl_twl_stgy_restart.restart_noGC[of _ U])
+      subgoal by (rule st)
+      subgoal using f unfolding m by simp
+      subgoal by (rule res)
+      done
+    show \<open>cdcl_twl_stgy_restart_with_leftovers (Ta, n, \<not>False) (?m V) (V, n, \<not>False)\<close>
+      unfolding not_False_eq_True cdcl_twl_stgy_restart_with_leftovers_def
+      by (rule exI[of _ \<open>V\<close>])(auto simp: twl_res_T_V)
+    show \<open>cdcl_twl_stgy_restart\<^sup>*\<^sup>* (S, 0, \<not>False) (V, n, \<not>False)\<close>
+      using twl_res twl_res_T_V TaT STa
+      unfolding cdcl_twl_stgy_restart_with_leftovers_def apply -
+      by auto
+    then show  \<open>cdcl_twl_stgy_restart_with_leftovers (S, 0, \<not>False) (?m V) (V, n, \<not>False)\<close>
+      unfolding cdcl_twl_stgy_restart_with_leftovers_def apply -
+      by (rule exI[of _ V]) auto
+    show \<open>cdcl_twl_stgy_restart_with_leftovers1 (Ta, n, \<not>False) (V, n, \<not>False)\<close>
+      using twl_res_T_V
+      unfolding cdcl_twl_stgy_restart_with_leftovers1_def not_False_eq_True
+      by fast
+  qed
+
+  have
+    rtranclp_twl_restart_after_restart_S_U:
+      \<open>cdcl_twl_stgy_restart_with_leftovers (S, 0, True) m (U, n, True)\<close> and
+    rtranclp_twl_restart_after_restart_T_U:
+      \<open>cdcl_twl_stgy_restart_with_leftovers (Ta, n, True) m (U, n, True)\<close>
+  proof -
+    have TaU: \<open>cdcl_twl_stgy\<^sup>*\<^sup>* Ta (fst (U, n))\<close>
+      using TaT \<open>cdcl_twl_stgy\<^sup>*\<^sup>* T U\<close> by auto
+    then show \<open>cdcl_twl_stgy_restart_with_leftovers (S, 0, True) m (U, n, True)\<close>
+      using STa m unfolding cdcl_twl_stgy_restart_with_leftovers_def
+      by fastforce
+    show \<open>cdcl_twl_stgy_restart_with_leftovers (Ta, n, True) m (U, n, True)\<close>
+      using \<open>cdcl_twl_stgy\<^sup>*\<^sup>* T U\<close> TaU m unfolding cdcl_twl_stgy_restart_with_leftovers_def
+      by fastforce
+  qed
+  have
+    rtranclp_twl_restart_after_restart_brk:
+      \<open>cdcl_twl_stgy_restart_with_leftovers (S, 0, True) m (U, n, True)\<close>
+    if
+      [simp]: \<open>brk = True\<close>
+  proof -
+    have \<open>full cdcl_twl_stgy T U \<or> get_conflict U \<noteq> None\<close>
+      using brk'_no_step \<open>cdcl_twl_stgy\<^sup>*\<^sup>* T U\<close>
+      unfolding rtranclp_unfold full_def final_twl_state_def by auto
+    then have \<open>(cdcl_twl_stgy\<^sup>*\<^sup>* T U \<and> pcdcl_twl_final_state U) \<or> get_conflict U \<noteq> None\<close>
+      unfolding full_def pcdcl_twl_final_state_def
+      by auto
+    then consider
+        (step) \<open>cdcl_twl_stgy_restart (T, n, True) (U, n, False)\<close> |
+        (final) \<open>get_conflict U \<noteq> None\<close>
+      using cdcl_twl_stgy_restart.intros(3)[of T U]
+      by (auto dest!: cdcl_twl_stgy_restart.intros)
+    then show \<open>cdcl_twl_stgy_restart_with_leftovers (S, 0, True) m (U, n, True)\<close>
+    proof cases
+      case step
+      then show ?thesis
+        using twl_res \<open>cdcl_twl_stgy\<^sup>*\<^sup>* T U\<close> unfolding cdcl_twl_stgy_restart_with_leftovers_def
+        using cdcl_twl_stgy_restart_cdcl_twl_stgy_cdcl_twl_stgy_restart2[of T n True U] apply -
+        by fastforce
+    next
+      case final
+      then show ?thesis
+        using twl_res \<open>cdcl_twl_stgy\<^sup>*\<^sup>* T U\<close>  unfolding cdcl_twl_stgy_restart_with_leftovers_def
+        by fastforce
+    qed
+  qed
+  have cdcl_twl_stgy_restart_with_leftovers1_T_U:
+    \<open>cdcl_twl_stgy_restart_with_leftovers1 (T, n, True) (U, n, True) \<longleftrightarrow> T \<noteq> U\<close>
+  proof -
+    have \<open>cdcl_twl_stgy\<^sup>+\<^sup>+ T U \<or> T = U\<close>
+      using \<open>cdcl_twl_stgy\<^sup>*\<^sup>* T U\<close> unfolding rtranclp_unfold by auto
+    then show ?thesis
+      using wf_not_refl[OF wf_cdcl_twl_stgy_restart, of \<open>(U, n, True)\<close>]
+      using wf_not_refl[OF tranclp_wf_cdcl_twl_stgy, of \<open>U\<close>]
+        struct_invs_U
+      unfolding cdcl_twl_stgy_restart_with_leftovers1_def by auto
+  qed
+  have brk'_eq: \<open>\<not>cdcl_twl_stgy_restart_with_leftovers1 (T, n, True) (U, n, True) \<Longrightarrow> brk'\<close>
+    using cdcl_o lits_to_upd_U lits_to_update local.cp
+    unfolding cdcl_twl_stgy_restart_with_leftovers1_def
+    unfolding rtranclp_unfold
+    by (auto dest!: tranclp_cdcl_twl_o_stgyD tranclp_cdcl_twl_cp_stgyD
+        simp: rtranclp_unfold
+        dest: rtranclp_tranclp_tranclp tranclp_trans)
+
+  have [simp]: \<open>brk = False\<close>
+    using cond by auto
+  show ?A
+    unfolding restart_prog_def restart_required_def
+    apply (refine_vcg; remove_dummy_vars)
+    subgoal using struct_invs_U stgy_invs_U confl_U unfolding restart_prog_pre_def by fast
+    subgoal using cdcl_twl_restart_only_twl_struct_invs struct_invs_U by blast
+    subgoal using cdcl_twl_stgy_restart_only_twl_stgy_invs stgy_invs_U by blast
+    subgoal by simp
+    subgoal by (rule cdcl_twl_stgy_restart_with_leftovers_after_restart_only)
+    subgoal by (auto simp add: cdcl_twl_restart_only.simps)
+    subgoal by (auto simp add: cdcl_twl_restart_only.simps)
+    subgoal apply (auto intro!: struct_invs_S struct_invs_T
+      cdcl_twl_stgy_restart_with_leftovers1_after_restart_only[unfolded not_False_eq_True])
+thm 
+  cdcl_twl_stgy_restart_with_leftovers1_after_restart_only[unfolded not_False_eq_True]
+
+      apply (rule 
+        cdcl_twl_stgy_restart_with_leftovers1_after_restart_only[unfolded not_False_eq_True])
       sorry
     subgoal by (rule struct_invs')
     subgoal by (rule stgy_invs)
